\documentclass[a4paper]{article}

\usepackage[utf8x]{inputenc}

\usepackage[left=4cm,top=3.5cm,right=4cm,bottom=3.5cm]{geometry}

\usepackage{geometry}
\geometry{a4paper}

\usepackage{graphicx}

\usepackage{minted}
% global minted style  
\setminted{  
encoding=utf-8
}

\usepackage{fancyhdr}

\pagestyle{fancy}
\fancyhf{}
\rhead{Palvinder Sander}
\lhead{Logic \& Computation Assessment One}
\rfoot{Page \thepage}

\usepackage{mathpartir}

\usepackage{bussproofs}
\usepackage{cancel}
\usepackage{tabularx}

%\usepackage{tcolorbox}
%\usepackage{etoolbox}
%\BeforeBeginEnvironment{minted}{\begin{tcolorbox}}%
%\AfterEndEnvironment{minted}{\end{tcolorbox}}%

\newminted{python}{frame=lines,framerule=2pt}

\title{Logic Assessment One}
\author{Palvinder Sander}
\date{}

\begin{document}

\section*{Question One:}

\subsection*{A)}
Corresponding lean proof:
\begin{minted}[frame=single,framesep=10pt,mathescape=true,escapeinside=||]{Lean}
theorem q1a (A B C : Prop) :
  |$(A \wedge C) \vee (B \wedge C) \rightarrow (A \vee B) \wedge C$| :=
assume h : |$(A \wedge C) \vee (B \wedge C)$|,
and.intro
  (or.elim h
    (assume k : |$A \wedge C$|, or.intro_left B (and.elim_left(k)))
    (assume l : |$B \wedge C$|, or.intro_right A (and.elim_left(l))))
  (or.elim h
    (assume k : |$A \wedge C$|, and.elim_right(k))
    (assume l : |$B \wedge C$|, and.elim_right(l)))
\end{minted}

\subsection*{B)}
Corresponding proof tree:
\begin{center}
\begin{prooftree}
\def\labelSpacing{3pt}
\def\extraVskip{3pt}
\def\ScoreOverhang{2pt}

\AxiomC{}
	\RightLabel{h}
	\UnaryInfC{$(A \wedge C) \vee (B \wedge C)$}
	
\AxiomC{}
	\RightLabel{k}
	\UnaryInfC{$A \wedge C$}
	\RightLabel{[$\wedge$E]}
	\UnaryInfC{$A,C$}
	\RightLabel{[$\vee$I]}
	\UnaryInfC{$A\vee B, A,C$}
	\RightLabel{[$\wedge$I]}
	\UnaryInfC{$(A \vee B) \wedge C$}
	\RightLabel{k[$\rightarrow$I]}
	\UnaryInfC{$A \rightarrow (A \vee B) \wedge C$}
	
\AxiomC{}
	\RightLabel{k}
	\UnaryInfC{$B \wedge C$}
	\RightLabel{[$\wedge$E]}
	\UnaryInfC{$B,C$}
	\RightLabel{[$\vee$I]}
	\UnaryInfC{$A\vee B, B,C$}
	\RightLabel{[$\wedge$I]}
	\UnaryInfC{$(A \vee B) \wedge C$}
	\RightLabel{k[$\rightarrow$I]}
	\UnaryInfC{$A \rightarrow (A \vee B) \wedge C$}
	\RightLabel{[$\vee E$]}
	
		\TrinaryInfC{$(A \vee B) \wedge C$}
		\RightLabel{h[$\rightarrow$I]}
		
			\UnaryInfC{$(A \wedge C) \vee (B \wedge C) \rightarrow (A \vee B) \wedge C$}
\end{prooftree}
\end{center}

\section*{Question Two:}
Truth table to check validity of the logical equivalence $(A \wedge C) \vee (B \wedge C) \leftrightarrow (A\vee B) \wedge C$:
\begin{table}[ht]
\centering
\def\arraystretch{1.5}
\begin{tabular}{|c|c|c|c|c|c|c|c|}
\hline
A & B & C & $A \wedge C$ & $B \wedge C$ & $(A \wedge C) \wedge (B \wedge C)$ & $(A \vee B)$ & $(A \vee B) \vee C$ \\ \hline
F & F & F & F & F & F & F & F \\
F & F & T & F & F & F & F & F \\
F & T & F & F & F & F & T & F \\
F & T & T & F & T & T & T & T \\
T & F & F & F & F & F & T & F \\
T & F & T & T & F & T & T & T \\
T & T & F & F & F & F & T & F \\
T & T & T & T & T & T & T & T \\ \hline
\end{tabular}
\end{table}

\section*{Question Three:}
\subsection*{A)}
Proof tree for proof of $A \rightarrow (A\wedge B)\vee(A \wedge \neg B)$ by natural deduction:
\begin{center}
\begin{prooftree}
\def\labelSpacing{3pt}
\def\extraVskip{3pt}
\def\ScoreOverhang{2pt}

\AxiomC{}
	\RightLabel{EM}
	\UnaryInfC{$B \vee \neg B$}
	
\AxiomC{}
	\RightLabel{x}
	\UnaryInfC{$A$}
	\RightLabel{y}
	\AxiomC{}
		\UnaryInfC{$B$}
	\RightLabel{[$\wedge$I]}
	\BinaryInfC{$A\wedge B$}
	\RightLabel{[$\vee$I]}
	\UnaryInfC{$(A \wedge B) \vee (A \wedge \neg B)$}
	\RightLabel{y[$\rightarrow$I]}
	\UnaryInfC{$B \rightarrow (A \wedge B) \vee (A \wedge \neg B)$}
	\RightLabel{[$\vee E$]}
	
\AxiomC{}
	\RightLabel{x}
	\UnaryInfC{$A$}
	\RightLabel{z}
	\AxiomC{}
		\UnaryInfC{$\neg B$}
	\RightLabel{[$\wedge$I]}
	\BinaryInfC{$A\wedge \neg B$}
	\RightLabel{[$\vee$I]}
	\UnaryInfC{$(A \wedge B) \vee (A \wedge \neg B)$}
	\RightLabel{z[$\rightarrow$I]}
	\UnaryInfC{$\neg B \rightarrow (A \wedge B) \vee (A \wedge \neg B)$}
	\RightLabel{[$\vee E$]}
	
		\TrinaryInfC{$(A \wedge B) \vee (A \wedge \neg B)$}
		\RightLabel{x[$\rightarrow$I]}
		
			\UnaryInfC{$A \rightarrow (A \wedge B) \vee (A \wedge \neg B)$}
\end{prooftree}
\end{center}
\subsection*{B)}
Proof implemented in lean:
\begin{minted}[frame=single,framesep=10pt,mathescape=true,escapeinside=||]{Lean}
open classical

theorem q3b (A B : Prop) :
  |$A \rightarrow (A \wedge B) \vee (A \wedge \neg B)$| :=
assume x : A,
or.elim (em B)
(assume y : B, or.intro_left |$(A \wedge \neg B)$| (and.intro(x)(y)))
(assume z : |$\neg$|B, or.intro_right |$(A \wedge B)$| (and.intro(x)(z)))
\end{minted}

\section*{Question 4:}
\subsection*{A)}
Expressing $P \wedge (Q \rightarrow R)$ in CNF form: \\
First we must create the corresponding truth table.
\begin{table}[ht]
\centering
\def\arraystretch{1.5}
\begin{tabular}{|c|c|c|c|c|c|c|c|}
\hline
P & Q & R & $P$ & $Q \rightarrow R$ & $P \wedge (Q \rightarrow R)$  \\ \hline
F & F & F & F & T & F  \\
F & F & T & F & T & F  \\
F & T & F & F & F & F  \\
F & T & T & F & T & F  \\
T & F & F & T & T & T  \\
T & F & T & T & T & T  \\
T & T & F & T & F & F  \\
T & T & T & T & T & T  \\ \hline
\end{tabular}
\end{table}
\newpage
Enumerating all the rows from the conclusion column.
\begin{enumerate}
\item $\neg P \wedge \neg Q \wedge \neg R$
\item $\neg P \wedge \neg Q \wedge R$
\item $\neg P \wedge Q \wedge \neg R$
\item $\neg P \wedge Q \wedge R$
\item $ P \wedge Q \wedge R$
\end{enumerate}
After negating these formulae (from only the $T$ rows) then joining them with an AND we get:
$$(P\vee Q \vee R) \wedge (P \vee Q \vee \neg R) \wedge (P \vee \neg Q \vee R) \wedge (P \vee \neg Q \vee \neg R) \wedge (\neg P \vee \neg Q \vee R)$$
\subsection*{B)}
Expressing $P \wedge (Q \rightarrow R)$ in DNF form:
First we must create the corresponding truth table.
\begin{table}[ht]
\centering
\def\arraystretch{1.5}
\begin{tabular}{|c|c|c|c|c|c|c|c|}
\hline
P & Q & R & $P$ & $Q \rightarrow R$ & $P \wedge (Q \rightarrow R)$  \\ \hline
F & F & F & F & T & F  \\
F & F & T & F & T & F  \\
F & T & F & F & F & F  \\
F & T & T & F & T & F  \\
T & F & F & T & T & T  \\
T & F & T & T & T & T  \\
T & T & F & T & F & F  \\
T & T & T & T & T & T  \\ \hline
\end{tabular}
\end{table}
\\Enumerating all the rows from the conclusion column.
\begin{enumerate}
\item $\neg P \wedge \neg Q \wedge \neg R$
\item $\neg P \wedge \neg Q \wedge R$
\item $\neg P \wedge Q \wedge \neg R$
\item $\neg P \wedge Q \wedge R$
\item $P \wedge Q \wedge R$
\end{enumerate}
After joining these formulae (from only the $T$ rows) with an OR we get:
$$(P \wedge \neg Q \wedge \neg R) \vee (P \wedge \neg Q \wedge R) \vee (P \wedge Q \wedge R)$$
\end{document}